Cslib/Computability/Languages/KleeneAlgorithm.lean
@@ -1,0 +1,189 @@
+/-
+Copyright (c) 2026 Brooke Gill and Chi-Yun Hsu. All rights reserved.
+Released under Apache 2.0 license as described in the file LICENSE.
+Authors: Brooke Gill and Chi-Yun Hsu
+-/
+
+module
+
+public import Cslib.Computability.Automata.Acceptors.Acceptor
+public import Cslib.Computability.Automata.DA.Basic
+public import Mathlib.Computability.RegularExpressions
+
+
+/-!
+# Kleene's Algorithm
+-/
+
+@[expose] public section
+
+namespace Cslib.Language
+
+open scoped FLTS
+
+variable {Symbol : Type*}
+
+section PathSupp
+
+variable {State : Type*}
+
+/-- PathSupp s xs is the set of states that can be reached from state s by reading the string xs,
+not including the starting state and the ending state. -/
+def PathSupp (flts : FLTS State Symbol) : State → List Symbol → Set State
+  | _, [] | _, [_] => ∅
+  | s, a :: x => {flts.tr s a} ∪ PathSupp flts (flts.tr s a) x
+
+theorem pathSupp_empty_iff_empty_or_char {flts : FLTS State Symbol} {s : State} {xs : List Symbol} :
+    PathSupp flts s xs = ∅ ↔ xs = [] ∨ (∃ a : Symbol, xs = [a]) := by
+  match xs with
+  | [] | [_] => grind [PathSupp]
+  | x :: y :: ys =>
+    have : flts.tr s x ∈ PathSupp flts s (x :: y :: ys) := by grind [PathSupp]
+    grind
+
+theorem pathSupp_head {flts : FLTS State Symbol} {s : State} {a : Symbol} {xs : List Symbol}
+    (hxs : xs ≠ []) : PathSupp flts s (a :: xs) =
+    {flts.tr s a} ∪ PathSupp flts (flts.tr s a) xs := by
+  grind [PathSupp]
+
+theorem pathSupp_append {flts : FLTS State Symbol} {s : State} {xs ys : List Symbol}
+    (hxs : xs ≠ [] ∧ ys ≠ []) : PathSupp flts s (xs ++ ys) =
+    {flts.mtr s xs} ∪ PathSupp flts s xs ∪ PathSupp flts (flts.mtr s xs) ys := by
+  induction xs generalizing s with
+  | nil => grind [PathSupp]
+  | cons a xs ih =>
+  rw [List.cons_append, pathSupp_head (by simp [hxs.2])]
+  by_cases hx : xs = []
+  · grind [PathSupp]
+  · grind [pathSupp_head hx]
+
+end PathSupp
+
+open Automata Acceptor
+
+/-- A Bounded Path (`BddPath`) has states `Fin n` and accepts strings (lists of symbols)
+starting with state `start` and ending with state `finish`
+with the intermediate states less than `bound`. -/
+structure BddPath (n : ℕ) (Symbol : Type*) extends FLTS (Fin n) Symbol where
+  start : Fin n
+  finish : Fin n
+  bound : ℕ
+
+instance {n : ℕ} : Acceptor (BddPath n Symbol) Symbol where
+  Accepts (a : BddPath n Symbol) (xs : List Symbol) :=
+    a.mtr a.start xs = a.finish ∧ (∀ i ∈ PathSupp a.toFLTS a.start xs, i < a.bound)
+
+theorem language_bddpath_head_iff {n k : ℕ} {flts : FLTS (Fin n) Symbol} {i j : Fin n}
+   {a : Symbol} {xs : List Symbol} :
+    a :: xs ∈ language (BddPath.mk flts i j k) ↔
+    xs ∈ language (BddPath.mk flts (flts.tr i a) j k) ∧ (flts.tr i a < k ∨ xs = []) := by
+  simp only [mem_language, Accepts]
+  by_cases hxs : xs = []
+  · grind [PathSupp]
+  grind [pathSupp_head hxs]
+
+theorem language_bddpath_eq_dfa {n k : ℕ} (flts : FLTS (Fin n) Symbol) (i j : Fin n) (hk : n ≤ k) :
+    language (BddPath.mk flts i j k) = language (DA.FinAcc.mk {tr := flts.tr, start := i} {j}) := by
+  ext xs
+  simp only [mem_language, Accepts]
+  grind
+
+section splitLast
+
+open List
+
+-- variable [DecidableEq Symbol]
+
+/-- The function `splitLast` sends a string to its shortest suffix starting at state `t`.
+If the string ends at state `t`, then `splitLast` returns the empty string.
+If the string never passes through state `t` (starting state can be `t`),
+then `splitLast` returns the original string. -/
+def splitLast [DecidableEq Symbol] {n : ℕ} (flts : FLTS (Fin n) Symbol) (s t : Fin n) :
+    List Symbol → List Symbol
+  | [] => []
+  | a :: x => if (splitLast flts (flts.tr s a) t x = x) ∧ flts.tr s a ≠ t then a :: x
+  else splitLast flts (flts.tr s a) t x
+
+theorem isSuffix_splitLast [DecidableEq Symbol] {n : ℕ} (flts : FLTS (Fin n) Symbol) (s t : Fin n)
+    (xs : List Symbol) : IsSuffix (splitLast flts s t xs) xs := by
+  induction xs generalizing s with
+  | nil => simp [splitLast]
+  | cons a xs ih => grind [splitLast]
+
+def splitLastCompl {n : ℕ} (flts : FLTS (Fin n) Symbol) (s t : Fin n) : List Symbol → List Symbol
+  | [] => []
+  | a :: x => if (splitLastCompl flts (flts.tr s a) t x = []) ∧ flts.tr s a ≠ t then []
+  else a :: splitLastCompl flts (flts.tr s a) t x
+
+theorem splitLast_append [DecidableEq Symbol] {n : ℕ} (flts : FLTS (Fin n) Symbol) (s t : Fin n)
+    (xs : List Symbol) : splitLastCompl flts s t xs ++ splitLast flts s t xs = xs := by
+  induction xs generalizing s with
+  | nil => grind [splitLast, splitLastCompl]
+  | cons a xs ih =>
+  simp only [splitLast, splitLastCompl]
+  split_ifs with h h' h'
+  · simp
+  · grind [ih (s := flts.tr s a)]
+  · have := h'.1 ▸ ih (s := flts.tr s a)
+    simp at this
+    grind
+  · simpa using ih (s := flts.tr s a)
+
+theorem splitLast_eq [DecidableEq Symbol] {n : ℕ} {flts : FLTS (Fin n) Symbol} {s t : Fin n}
+    {xs : List Symbol} (h : t ∉ PathSupp flts s xs) (h' : t = flts.mtr s xs) :
+    splitLast flts s t xs = [] := by
+  induction xs generalizing s with
+  | nil => grind [splitLast, PathSupp]
+  | cons a xs ih =>
+  by_cases hxs : xs = []
+  · grind [splitLast, PathSupp]
+  rw [pathSupp_head hxs, Set.mem_union, Set.mem_singleton_iff] at h
+  grind [splitLast, (isSuffix_splitLast flts (flts.tr s a) t xs).length_le]
+
+theorem splitLastCompl_eq {n : ℕ} {flts : FLTS (Fin n) Symbol} {s t : Fin n}
+    {xs : List Symbol} (h : t ∉ PathSupp flts s xs) (h' : t = flts.mtr s xs) :
+    splitLastCompl flts s t xs = xs := by
+  classical
+  simpa [splitLast_eq h h'] using splitLast_append flts s t xs
+
+theorem splitLast_neq_iff_mem_PathSupp [DecidableEq Symbol] {n : ℕ} {flts : FLTS (Fin n) Symbol}
+   {s t : Fin n} {xs : List Symbol} (hxs : xs ≠ []) :
+    ¬(splitLast flts s t xs = xs) ↔ t ∈ PathSupp flts s xs ∨ t = flts.mtr s xs := by
+  induction xs generalizing s with
+  | nil => contradiction
+  | cons a xs ih =>
+  by_cases hxs' : xs = []
+  · grind [splitLast, PathSupp]
+  rw [pathSupp_head hxs', Set.mem_union, Set.mem_singleton_iff]
+  grind [splitLast, (isSuffix_splitLast flts (flts.tr s a) t xs).length_le]
+
+theorem splitLastCompl_nonempty_iff_mem_PathSupp {n : ℕ} {flts : FLTS (Fin n) Symbol}
+   {s t : Fin n} {xs : List Symbol} (hxs : xs ≠ []) :
+    ¬(splitLastCompl flts s t xs = []) ↔ t ∈ PathSupp flts s xs ∨ t = flts.mtr s xs := by
+  classical
+  rw [← splitLast_neq_iff_mem_PathSupp hxs, not_iff_not]
+  nth_rw 3 [← splitLast_append flts s t xs]
+  simp
+
+end splitLast
+
+/-
+Regex i j k is the regex for the path from state i to state j passing through states < k.
+When k = 0, i = j, the regex is ε union all characters from state i to state i.
+When k = 0, i ≠ j, the regex is all characters from state i to state j.
+For k + 1, the regex is the union of Regex i j k and
+(Regex i k k) (Regex k k k)∗ (Regex k j k).
+-/
+noncomputable def Regex [Fintype Symbol] {n : ℕ} (flts : FLTS (Fin n) Symbol)
+    (i j : Fin n) : ℕ → RegularExpression Symbol
+  | 0 =>
+    let chars := (Finset.univ.filter
+      (fun x : Symbol ↦ flts.tr i x = j)).toList.map RegularExpression.char
+    if i = j then 1 + chars.sum else chars.sum
+  | k + 1 =>
+    if h : n ≤ k then Regex flts i j k
+    else
+      let kFin : Fin n := ⟨k, by omega⟩
+      Regex flts i j k + Regex flts i kFin k * (Regex flts kFin kFin k).star * Regex flts kFin j k
+
+end Cslib.Language
